ROOT
@@ -7,7 +7,7 @@ session "UTP-Angelic-Designs" in "angelic-designs" = "UTP-Reactive-Designs" +
     utp_ades_designs
     utp_ades
 
-session "UTP-Angelic-CSP" = "UTP-Angelic-Designs" +
+session "UTP-Reactive-Angelic-Designs" in "reactive-angelic-designs" = "UTP-Angelic-Designs" +
   options [document = false]
   theories
     utp_rad_core
@@ -19,4 +19,9 @@ session "UTP-Angelic-CSP" = "UTP-Angelic-Designs" +
     utp_rad_examples
     utp_rad_nd
     utp_rad
+
+session "UTP-Angelic-CSP" = "UTP-Reactive-Angelic-Designs" +
+  options [document = false]
+  theories
+    utp_ap_healthy
     Angelic_CSP
